Add call events in the frontend

backend/Cminor.v
@@ -468,7 +468,7 @@ Inductive step: state -> trace -> state -> Prop :=
       step (State f (Sstore chunk addr a) k sp e m)
         E0 (State f Sskip k sp e m')
 
-  | step_call: forall f optid sig a bl k sp e m vf vargs fd,
+  | step_call: forall f optid sig a bl k sp e m vf vargs fd t,
       eval_expr sp e m (comp_of f) a vf ->
       eval_exprlist sp e m (comp_of f) bl vargs ->
       Genv.find_funct ge vf = Some fd ->
@@ -476,10 +476,11 @@ Inductive step: state -> trace -> state -> Prop :=
       (* Check that the call to the function pointer is allowed *)
       forall (ALLOWED: Genv.allowed_call ge (comp_of f) vf),
       forall (NO_CROSS_PTR: Genv.type_of_call ge (comp_of f) (Genv.find_comp ge vf) = Genv.CrossCompartmentCall -> Forall not_ptr vargs),
+      forall (EV: call_trace ge (comp_of f) (Genv.find_comp ge vf) vf vargs (sig_args sig) t),
       step (State f (Scall optid sig a bl) k sp e m)
-        E0 (Callstate fd vargs (Kcall optid f sp e k) m)
+        t (Callstate fd vargs (Kcall optid f sp e k) m)
 
-  | step_tailcall: forall f sig a bl k sp e m vf vargs fd m',
+  | step_tailcall: forall f sig a bl k sp e m vf vargs fd m' t,
       eval_expr (Vptr sp Ptrofs.zero) e m (comp_of f) a vf ->
       eval_exprlist (Vptr sp Ptrofs.zero) e m (comp_of f) bl vargs ->
       Genv.find_funct ge vf = Some fd ->
@@ -488,8 +489,9 @@ Inductive step: state -> trace -> state -> Prop :=
       forall (ALLOWED: needs_calling_comp (comp_of f) = false),
       forall (ALLOWED': Genv.allowed_call ge (comp_of f) vf),
       Mem.free m sp 0 f.(fn_stackspace) (comp_of f) = Some m' ->
+      forall (EV: call_trace ge (comp_of f) (Genv.find_comp ge vf) vf vargs (sig_args sig) t),
       step (State f (Stailcall sig a bl) k (Vptr sp Ptrofs.zero) e m)
-        E0 (Callstate fd vargs (call_cont k) m')
+        t (Callstate fd vargs (call_cont k) m')
 
   | step_builtin: forall f optid ef bl k sp e m vargs t vres m',
       eval_exprlist sp e m (comp_of f) bl vargs ->
@@ -602,12 +604,16 @@ Proof.
   assert (t1 = E0 -> exists s2, step (Genv.globalenv p) s t2 s2).
     intros. subst. inv H0. exists s1; auto.
   inversion H; subst; auto.
+  inv EV; inv H0; eexists; eauto.
+  inv EV; inv H0; eexists; eauto.
   exploit external_call_receptive; eauto. intros [vres2 [m2 EC2]].
   exists (State f Sskip k sp (set_optvar optid vres2 e) m2). econstructor; eauto.
   exploit external_call_receptive; eauto. intros [vres2 [m2 EC2]].
   exists (Returnstate vres2 k m2 (comp_of ef)). econstructor; eauto.
 (* trace length *)
-  red; intros; inv H; simpl; try omega; eapply external_call_trace_length; eauto.
+  red; intros; inv H; simpl; try omega; try now eapply external_call_trace_length; eauto.
+  inv EV; auto.
+  inv EV; auto.
 Qed.
 
 (** This semantics is determinate. *)
@@ -659,6 +665,22 @@ Proof.
   intros. constructor; set (ge := Genv.globalenv p); simpl; intros.
 - (* determ *)
   inv H; inv H0; Determ.
+  + subst. rewrite H16 in H3; inv H3.
+    inv EV; inv EV0; try congruence.
+    split; [constructor | auto].
+    inv H3; auto.
+    assert (i0 = i) by congruence; subst.
+    assert (vl0 = vl) by now eapply eventval_list_match_determ_2; eauto. subst.
+    split; [constructor | auto].
+  + subst.
+    rewrite H16 in H3; inv H3.
+    rewrite H18 in H5; inv H5.
+    inv EV; inv EV0; try congruence.
+    split; [constructor | auto].
+    inv H3; auto.
+    assert (i0 = i) by congruence; subst.
+    assert (vl0 = vl) by now eapply eventval_list_match_determ_2; eauto. subst.
+    split; [constructor | auto].
   + subst vargs0. exploit external_call_determ. eexact H2.  eexact H13.
     intros (A & B). split; intros; auto.
     apply B in H; destruct H; congruence.
@@ -669,7 +691,8 @@ Proof.
     apply B in H; destruct H; congruence.
 - (* single event *)
   red; simpl. destruct 1; simpl; try omega;
-  eapply external_call_trace_length; eauto.
+  try now eapply external_call_trace_length; eauto.
+  inv EV; auto. inv EV; auto.
 - (* initial states *)
   inv H; inv H0. unfold ge0, ge1 in *. congruence.
 - (* nostep final state *)
@@ -781,7 +804,7 @@ with exec_stmt:
       Mem.storev chunk m vaddr v (comp_of f) = Some m' ->
       exec_stmt f sp e m (Sstore chunk addr a) E0 e m' Out_normal
   | exec_Scall:
-      forall f sp e m optid sig a bl vf vargs fd t m' vres e',
+      forall f sp e m optid sig a bl vf vargs fd t m' vres e' t',
       eval_expr ge sp e m (comp_of f) a vf ->
       eval_exprlist ge sp e m (comp_of f) bl vargs ->
       Genv.find_funct ge vf = Some fd ->
@@ -790,8 +813,9 @@ with exec_stmt:
       e' = set_optvar optid vres e ->
       forall (ALLOWED: Genv.allowed_call ge (comp_of f) vf),
       forall (NO_CROSS_PTR_CALL: Genv.type_of_call ge (comp_of f) (Genv.find_comp ge vf) = Genv.CrossCompartmentCall -> Forall not_ptr vargs),
+      forall (EV: call_trace ge (comp_of f) (Genv.find_comp ge vf) vf vargs (sig_args sig) t'),
       forall (NO_CROSS_PTR_RETURN: Genv.type_of_call ge (comp_of f) (Genv.find_comp ge vf) = Genv.CrossCompartmentCall -> not_ptr vres),
-      exec_stmt f sp e m (Scall optid sig a bl) t e' m' Out_normal
+      exec_stmt f sp e m (Scall optid sig a bl) (t' ** t) e' m' Out_normal
   | exec_Sbuiltin:
       forall f sp e m optid ef bl t m' vargs vres e',
       eval_exprlist ge sp e m (comp_of f) bl vargs ->
@@ -847,7 +871,7 @@ with exec_stmt:
       eval_expr ge sp e m (comp_of f) a v ->
       exec_stmt f sp e m (Sreturn (Some a)) E0 e m (Out_return (Some v))
   | exec_Stailcall:
-      forall f sp e m sig a bl vf vargs fd t m' m'' vres,
+      forall f sp e m sig a bl vf vargs fd t m' m'' vres t',
       eval_expr ge (Vptr sp Ptrofs.zero) e m (comp_of f) a vf ->
       eval_exprlist ge (Vptr sp Ptrofs.zero) e m (comp_of f) bl vargs ->
       Genv.find_funct ge vf = Some fd ->
@@ -857,7 +881,8 @@ with exec_stmt:
       forall (ALLOWED': Genv.allowed_call ge (comp_of f) vf),
       Mem.free m sp 0 f.(fn_stackspace) (comp_of f) = Some m' ->
       eval_funcall (comp_of f) m' fd vargs t m'' vres ->
-      exec_stmt f (Vptr sp Ptrofs.zero) e m (Stailcall sig a bl) t e m'' (Out_tailcall_return vres).
+      forall (EV: call_trace ge (comp_of f) (Genv.find_comp ge vf) vf vargs (sig_args sig) t'),
+      exec_stmt f (Vptr sp Ptrofs.zero) e m (Stailcall sig a bl) (t' ** t) e m'' (Out_tailcall_return vres).
 
 Scheme eval_funcall_ind2 := Minimality for eval_funcall Sort Prop
   with exec_stmt_ind2 := Minimality for exec_stmt Sort Prop.
@@ -887,7 +912,7 @@ CoInductive evalinf_funcall:
 with execinf_stmt:
          function -> val -> env -> mem -> stmt -> traceinf -> Prop :=
   | execinf_Scall:
-      forall f sp e m optid sig a bl vf vargs fd t,
+      forall f sp e m optid sig a bl vf vargs fd t t',
       eval_expr ge sp e m (comp_of f) a vf ->
       eval_exprlist ge sp e m (comp_of f) bl vargs ->
       Genv.find_funct ge vf = Some fd ->
@@ -895,7 +920,8 @@ with execinf_stmt:
       evalinf_funcall m fd vargs t ->
       forall (ALLOWED: Genv.allowed_call ge (comp_of f) vf),
       forall (NO_CROSS_PTR: Genv.type_of_call ge (comp_of f) (Genv.find_comp ge vf) = Genv.CrossCompartmentCall -> Forall not_ptr vargs),
-      execinf_stmt f sp e m (Scall optid sig a bl) t
+      forall (EV: call_trace ge (comp_of f) (Genv.find_comp ge vf) vf vargs (sig_args sig) t'),
+      execinf_stmt f sp e m (Scall optid sig a bl) (t' *** t)
   | execinf_Sifthenelse:
       forall f sp e m a s1 s2 v b t,
       eval_expr ge sp e m (comp_of f) a v ->
@@ -927,7 +953,7 @@ with execinf_stmt:
       execinf_stmt f sp e m s t ->
       execinf_stmt f sp e m (Sblock s) t
   | execinf_Stailcall:
-      forall f sp e m sig a bl vf vargs fd m' t,
+      forall f sp e m sig a bl vf vargs fd m' t t',
       eval_expr ge (Vptr sp Ptrofs.zero) e m (comp_of f) a vf ->
       eval_exprlist ge (Vptr sp Ptrofs.zero) e m (comp_of f) bl vargs ->
       Genv.find_funct ge vf = Some fd ->
@@ -937,7 +963,8 @@ with execinf_stmt:
       forall (ALLOWED': Genv.allowed_call ge (comp_of f) vf),
       Mem.free m sp 0 f.(fn_stackspace) (comp_of f) = Some m' ->
       evalinf_funcall  m' fd vargs t ->
-      execinf_stmt f (Vptr sp Ptrofs.zero) e m (Stailcall sig a bl) t.
+      forall (EV: call_trace ge (comp_of f) (Genv.find_comp ge vf) vf vargs (sig_args sig) t'),
+      execinf_stmt f (Vptr sp Ptrofs.zero) e m (Stailcall sig a bl) (t' *** t).
 
 End NATURALSEM.
 
