cfrontend/Csharpminor.v
@@ -393,15 +393,16 @@ Inductive step: state -> trace -> state -> Prop :=
       step (State f (Sstore chunk addr a) k e le m)
         E0 (State f Sskip k e le m')
 
-  | step_call: forall f optid sig a bl k e le m vf vargs fd,
+  | step_call: forall f optid sig a bl k e le m vf vargs fd t,
       eval_expr e (comp_of f) le m a vf ->
       eval_exprlist e (comp_of f) le m bl vargs ->
       Genv.find_funct ge vf = Some fd ->
       funsig fd = sig ->
       forall (ALLOWED: Genv.allowed_call ge (comp_of f) vf),
       forall (NO_CROSS_PTR: Genv.type_of_call ge (comp_of f) (Genv.find_comp ge vf) = Genv.CrossCompartmentCall -> Forall not_ptr vargs),
+      forall (EV: call_trace ge (comp_of f) (Genv.find_comp ge vf) vf vargs (sig_args sig) t),
       step (State f (Scall optid sig a bl) k e le m)
-        E0 (Callstate fd vargs (Kcall optid f e le k) m)
+        t (Callstate fd vargs (Kcall optid f e le k) m)
 
   | step_builtin: forall f optid ef bl k e le m vargs t vres m',
       eval_exprlist e (comp_of f) le m bl vargs ->
